src/Prog.v
@@ -62,11 +62,19 @@ Inductive prog (T: Type) :=
 | Sync (a: addr) (rx: unit -> prog T).
 
 Definition progseq (A B:Type) (a:B->A) (b:B) := a b.
+Definition pair_args_helper (A B C:Type) (f: A->B->C) (x: A*B) := f (fst x) (snd x).
+Notation "^( a )" := (pair a I).
+Notation "^( a , .. , b )" := (pair a .. (pair b I) ..).
 
 Notation "p1 ;; p2" := (progseq p1 (fun _: unit => p2)) (at level 60, right associativity).
 Notation "x <- p1 ; p2" := (progseq p1 (fun x => p2)) (at level 60, right associativity).
-Notation "'let2' ( a , b ) <- p1 ; p2" := (progseq p1 (fun x => let (a, b) := x in p2)) (at level 60, right associativity).
-Notation "'let3' ( a , b , c ) <- p1 ; p2" := (progseq p1 (fun y => let (x, c) := y in let (a, b) := x in p2)) (at level 60, right associativity).
+Notation "'let^' ( a , .. , b ) <- p1 ; p2" :=
+  (progseq p1
+    (pair_args_helper (fun a => ..
+      (pair_args_helper (fun b (_:True) => p2))
+    ..))
+  )
+  (at level 60, right associativity, a closed binder, b closed binder).
 
 
 Definition DecEq (T : Type) := forall (a b : T), {a=b}+{a<>b}.
